theorems/iN/iN_rewrite.lean
@@ -1,0 +1,44 @@
+import theorems.iN.iN_def
+
+/--
+`Rewrite x y` means the value `x` can be rewritten into the value `y`.
+-/
+inductive Rewrite {n} : iN n → iN n → Prop where
+  /-- A non-poison value rewrites to itself. -/
+  | bv_refl (v : BitVec n) : Rewrite (bitvec v) (bitvec v)
+  /-- Poison can be rewritten into any value. -/
+  | poison_forge (v : BitVec n) : Rewrite poison (bitvec v)
+
+/--
+`RewriteReverse x y` means the value `y` can be rewritten into the value `x`.
+-/
+abbrev RewriteReverse {n} (x y : iN n) := Rewrite y x
+
+/--
+`RewriteIff x y` means `x` can be rewritten into `y` and `y` can be rewritten into `x`.
+-/
+abbrev RewriteIff {n} (x y : iN n) := Rewrite x y ∧ Rewrite y x
+
+@[inherit_doc] infix:50 " ~> "  => Rewrite
+@[inherit_doc] infix:50 " <~ "  => RewriteReverse
+@[inherit_doc] infix:50 " <~> " => RewriteIff
+
+/- theorem rewrite_bitvec_iff_equal {n} {x y : BitVec n}
+    : (bitvec x <~> bitvec y) ↔ (x = y) := by
+
+  constructor
+  case mp =>
+    intro h
+    cases h with
+    | intro hxy hyx =>
+      cases hxy
+      cases hyx
+      rfl
+  case mpr =>
+    intro h
+    rw [h]
+    constructor
+    case left => exact Rewrite.bv_refl y
+    case right => exact Rewrite.bv_refl y -/
+
+-- you can have `poison ~> 12`
