theorems/iN/iN_tactics.lean
@@ -1,0 +1,12 @@
+import Lean
+
+open Lean Elab Tactic Meta
+
+/- elab "lift_poison" : tactic =>
+  Tactic.withMainContext do
+    let goalType ← Lean.Elab.Tactic.getMainTarget
+    dbg_trace f!"goal type: {goalType}"
+
+
+    goalType.eq
+ -/
